Use height instead of Repr for termination, split up more files

src/Actions/Actions.dfy
@@ -11,7 +11,7 @@ module Actions {
   import opened Seq
   import opened Math
 
-  trait Action<T, R> extends Validatable {
+  trait {:termination false} Action<T, R> extends Validatable {
 
     ghost var consumed: seq<T>
     ghost var produced: seq<R>
@@ -21,12 +21,14 @@ module Actions {
       ensures Valid() ==> this in Repr 
       ensures Valid() ==> 
         && CanProduce(consumed, produced)
-      decreases Repr, 0
-    
+      decreases height, 0
+
     ghost predicate CanConsume(consumed: seq<T>, produced: seq<R>, next: T)
       requires CanProduce(consumed, produced)
+      decreases height
 
     ghost predicate CanProduce(consumed: seq<T>, produced: seq<R>)
+      decreases height
 
     ghost method Update(t: T, r: R) 
       modifies `consumed, `produced
@@ -41,12 +43,9 @@ module Actions {
       requires Valid()
       requires CanConsume(consumed, produced, t)
       modifies Repr
-      decreases Repr
+      decreases height
       ensures Valid()
-      // TODO: Will cause trouble when composing, see FilteredEnumerator in Enumerators.dfy
-      // ensures fresh(Repr - old(Repr))
-      // TODO: Not compatible with all actions
-      ensures Repr <= old(Repr)
+      ensures fresh(Repr - old(Repr))
       ensures consumed == old(consumed) + [t]
       ensures produced == old(produced) + [r]
       ensures CanProduce(consumed, produced)
@@ -59,265 +58,13 @@ module Actions {
       i.CanProduce(consumed, toProduce) <==> forall x <- toProduce :: x == c
   }
 
-  ghost predicate TerminatedBy<T>(s: seq<T>, c: T) {
-    forall i, j | 0 <= i < j < |s| :: s[i] == c ==> s[j] == c
+  ghost predicate Terminated<T>(s: seq<T>, c: T, n: nat) {
+    forall i | 0 <= i < |s| :: n <= i <==> s[i] == c
   }
 
-  ghost predicate TerminatedByBeyond<T>(s: seq<T>, c: T, n: nat) {
-    forall i | n <= i < |s| :: s[i] == c
-  }
-
-  function Enumerated<T>(produced: seq<Option<T>>): seq<T> {
-    if |produced| == 0 || produced[0].None? then
-      []
-    else
-      [produced[0].value] + Enumerated(produced[1..])
-  }
-
-  lemma TerminatedByBoundsEnumerated<T>(s: seq<Option<T>>, n: nat) 
-    requires TerminatedByBeyond(s, None, n)
-    ensures |Enumerated(s)| <= n
-  {
-    if |s| == 0 || s[0].None? {
-    } else {
-      TerminatedByBoundsEnumerated(s[1..], n - 1);
-    }
-  }
-
-  ghost function ProducedForEnumerator<T>(s: seq<T>, n: nat): seq<Option<T>> {
-    var before := Math.Min(|s|, n);
-    var after := Math.Max(|s|, n);
-    Seq.Map(x => Some(x), s[..before]) + Seq.Repeat(None, after - before)
-  }
-
-  ghost predicate EnumeratesAtMost<T(!new)>(e: Action<(), Option<T>>, n: nat) {
-    forall consumed: seq<()>, toProduce: seq<Option<T>> ::
-      e.CanProduce(consumed, toProduce) ==> |Enumerated(toProduce)| <= n
-  }
-
-  
-
-  ghost predicate ProducesTerminatedBy<T(!new), R(!new)>(i: Action<T, R>, c: R, n: nat) {
-    forall consumed: seq<T>, toProduce: seq<R> ::
-      i.CanProduce(consumed, toProduce) ==> TerminatedByBeyond(toProduce, c, n)
-  }
-
-  ghost predicate ConsumesAnything<T(!new)>(a: Action<(), Option<T>>) {
-    forall consumed, produced, next | a.CanProduce(consumed, produced) :: a.CanConsume(consumed, produced, next)
-  }
-
-  ghost predicate IsEnumerator<T(!new)>(a: Action<(), Option<T>>) {
-    ConsumesAnything(a) && exists n :: ProducesTerminatedBy(a, None, n)
-  }
-
-  ghost function EnumerationDecreases<T(!new)>(a: Action<(), Option<T>>): nat
-    requires a.Valid()
-    reads a.Repr
-    requires IsEnumerator(a)
-  {
-    var limit: nat :| ProducesTerminatedBy(a, None, limit);
-    TerminatedByBoundsEnumerated(a.produced, limit);
-    limit - |Enumerated(a.produced)|
-  }
-
-  // Potentially infinite enumerator
-  type IEnumerator<T> = Action<(), T> 
-
-  class SeqEnumerator<T> extends Action<(), Option<T>> {
-
-    const elements: seq<T>
-    // TODO: size_t? It's a hell of a lot easier to prove correct
-    // if this can increase unbounded to stay at |consumed|,
-    // but it's not ghost so we care about bounding it.
-    var index: nat
-
-    ghost predicate Valid() 
-      reads this, Repr 
-      ensures Valid() ==> this in Repr 
-      ensures Valid() ==> 
-        && CanProduce(consumed, produced)
-      decreases Repr, 0
-    {
-      && this in Repr
-      && index == |consumed|
-      && CanProduce(consumed, produced)
-    }
-
-    constructor(s: seq<T>) 
-      ensures Valid()
-      ensures fresh(Repr - {this})
-      ensures produced == []
-      ensures elements == s
-    {
-      elements := s;
-      index := 0;
-      
-      consumed := [];
-      produced := [];
-      Repr := {this};
-    }
-
-    ghost predicate CanConsume(consumed: seq<()>, produced: seq<Option<T>>, next: ()) {
-      true
-    }
-    ghost predicate CanProduce(consumed: seq<()>, produced: seq<Option<T>>) {
-      var index := |consumed|;
-      var values := Math.Min(index, |elements|);
-      var nones := index - values;
-      produced == Seq.Map(x => Some(x), elements[..values]) + Seq.Repeat(None, nones)
-    }
-
-    method Invoke(t: ()) returns (r: Option<T>) 
-      requires Valid()
-      requires CanConsume(consumed, produced, t)
-      modifies Repr
-      decreases Repr
-      ensures Valid()
-      ensures Repr <= old(Repr)
-      ensures consumed == old(consumed) + [t]
-      ensures produced == old(produced) + [r]
-      ensures CanProduce(consumed, produced)
-    {
-      if index < |elements| {
-        r := Some(elements[index]);
-      } else {
-        r := None;
-      }
-
-      index := index + 1;
-      Update((), r);
-    }
-  }
-
-  lemma SeqEnumeratorIsEnumerator<T(!new)>(e: SeqEnumerator<T>) 
-    ensures IsEnumerator(e)
-  {
-    assert ProducesTerminatedBy(e, None, |e.elements|);
-  }
-
-  class SeqIEnumerator<T> extends Action<(), T> {
-
-    const elements: seq<T>
-    var index: nat
-
-    ghost predicate Valid() 
-      reads this, Repr 
-      ensures Valid() ==> this in Repr 
-      ensures Valid() ==> 
-        && CanProduce(consumed, produced)
-      decreases Repr, 0
-    {
-      && this in Repr
-      && 0 <= index <= |elements|
-      && |consumed| == index
-      && produced == elements[0..index]
-    }
-
-    constructor(s: seq<T>) 
-      ensures Valid()
-      ensures fresh(Repr - {this})
-      ensures produced == []
-      ensures elements == s
-    {
-      elements := s;
-      index := 0;
-      
-      consumed := [];
-      produced := [];
-      Repr := {this};
-    }
-
-    ghost predicate CanConsume(consumed: seq<()>, produced: seq<T>, next: ()) {
-      |consumed| + 1 <= |elements|
-    }
-    ghost predicate CanProduce(consumed: seq<()>, produced: seq<T>) {
-      |consumed| <= |elements| && produced == elements[..|consumed|]
-    }
-
-    method Invoke(t: ()) returns (r: T) 
-      requires Valid()
-      requires CanConsume(consumed, produced, t)
-      modifies Repr
-      decreases Repr
-      ensures Valid()
-      ensures Repr <= old(Repr)
-      ensures consumed == old(consumed) + [t]
-      ensures produced == old(produced) + [r]
-      ensures CanProduce(consumed, produced)
-    {
-      r := elements[index];
-      index := index + 1;
-
-      Update((), r);
-    }
-  }
-
-  class Filter<T(!new)> extends Action<(), Option<T>> {
-
-    const wrapped: Action<(), Option<T>>
-      
-    // TODO: Can we support --> or ~>?
-    const filter: T -> bool
-
-    ghost predicate Valid() 
-      reads this, Repr 
-      ensures Valid() ==> this in Repr 
-      ensures Valid() ==> 
-        && CanProduce(consumed, produced)
-      decreases Repr, 0
-    {
-      && this in Repr
-      && ValidComponent(wrapped)
-      && IsEnumerator(wrapped)
-      && CanProduce(consumed, produced)
-    }
-
-    constructor(filter: T -> bool, wrapped: Action<(), Option<T>>) 
-      requires wrapped.Valid()
-      requires IsEnumerator(wrapped)
-      requires wrapped.consumed == [] && wrapped.produced == []
-      ensures Valid()
-    { 
-      this.filter := filter;
-      this.wrapped := wrapped;
-
-      consumed := [];
-      produced := [];
-      Repr := {this} + wrapped.Repr;
-    }
-
-    ghost predicate CanConsume(consumed: seq<()>, produced: seq<Option<T>>, next: ()) {
-      true
-    }
-    ghost predicate CanProduce(consumed: seq<()>, produced: seq<Option<T>>) {
-      exists producedByWrapped: seq<Option<T>> ::
-        && wrapped.CanProduce(Seq.Repeat((), |producedByWrapped|), producedByWrapped)
-        && Enumerated(produced) == Seq.Filter(filter, Enumerated(producedByWrapped))
-    }
-
-    method Invoke(t: ()) returns (r: Option<T>) 
-      requires Valid()
-      requires CanConsume(consumed, produced, t)
-      modifies Repr
-      decreases Repr
-      ensures Valid()
-      ensures Repr <= old(Repr)
-      ensures consumed == old(consumed) + [t]
-      ensures produced == old(produced) + [r]
-      ensures CanProduce(consumed, produced)
-    {
-      assert Enumerated(produced) == Seq.Filter(filter, Enumerated(wrapped.produced));
-      r := wrapped.Invoke(());
-      while r.Some? && !filter(r.value)
-        invariant Valid()
-        invariant Enumerated(produced) == Seq.Filter(filter, Enumerated(wrapped.produced))
-        decreases EnumerationDecreases(wrapped)
-      {
-        r := wrapped.Invoke(());
-      }
-
-      Update(t, r);
-    }
+  ghost predicate ProducesTerminatedBy<T(!new), R(!new)>(i: Action<T, R>, c: R, limit: nat) {
+    forall consumed: seq<T>, produced: seq<R> ::
+      i.CanProduce(consumed, produced) ==> exists n: nat | n <= limit :: Terminated(produced, c, n)
   }
 
   // class Compose<T, V(!new), R> extends Action<T, R> {
@@ -396,7 +143,7 @@ module Actions {
       ensures Valid() ==> this in Repr 
       ensures Valid() ==> 
         && CanProduce(consumed, produced)
-      decreases Repr, 0
+      decreases height, 0
     {
       && this in Repr
       && storage in Repr
@@ -419,10 +166,14 @@ module Actions {
       Repr := {this, storage};
     }
 
-    ghost predicate CanConsume(consumed: seq<T>, produced: seq<()>, next: T) {
+    ghost predicate CanConsume(consumed: seq<T>, produced: seq<()>, next: T)
+      decreases height
+    {
       true
     }
-    ghost predicate CanProduce(consumed: seq<T>, produced: seq<()>) {
+    ghost predicate CanProduce(consumed: seq<T>, produced: seq<()>)
+      decreases height
+    {
       produced == Seq.Repeat((), |consumed|)
     }
 
@@ -434,7 +185,7 @@ module Actions {
       requires Valid()
       requires CanConsume(consumed, produced, t)
       modifies Repr
-      decreases Repr
+      decreases height
       ensures Valid()
       ensures fresh(Repr - old(Repr))
       ensures consumed == old(consumed) + [t]
@@ -516,22 +267,7 @@ module Actions {
   //   }
   // }
 
-
-
-  method Main() {
-    var e: Action<(), int> := new SeqIEnumerator([1, 2, 3, 4, 5]);
-    var x := e.Invoke(());
-    assert e.produced == [1];
-    x := e.Invoke(());
-    assert e.produced == [1, 2];
-    x := e.Invoke(());
-    assert e.produced == [1, 2, 3];
-    x := e.Invoke(());
-    assert e.produced == [1, 2, 3, 4];
-    x := e.Invoke(());
-    assert e.produced == [1, 2, 3, 4, 5];
-
-
+  method AggregatorExample() {
     var a := new ArrayAggregator();
     var _ := a.Invoke(1);
     var _ := a.Invoke(2);
