src/Actions/FilteredEnumerator.dfy
@@ -1,0 +1,112 @@
+
+include "Enumerators.dfy"
+
+module Filtered {
+
+  import opened Actions
+  import opened Enumerators
+  import opened Wrappers
+  import opened Seq
+
+  class Filter<T(!new)> extends Action<(), Option<T>> {
+
+    const wrapped: Action<(), Option<T>>
+    ghost const wrappedCanProduce: (seq<()>, seq<Option<T>>) -> bool
+      
+    // TODO: Can we support --> or ~>?
+    const filter: T -> bool
+
+    ghost predicate Valid() 
+      reads this, Repr 
+      ensures Valid() ==> this in Repr 
+      ensures Valid() ==> 
+        && CanProduce(consumed, produced)
+      decreases height, 0
+    {
+      && this in Repr
+      && ValidComponent(wrapped)
+      && IsEnumerator(wrapped)
+      && CanProduce(consumed, produced)
+      && Enumerated(produced) == Seq.Filter(filter, Enumerated(wrapped.produced))
+    }
+
+    constructor(filter: T -> bool, wrapped: Action<(), Option<T>>) 
+      requires wrapped.Valid()
+      requires IsEnumerator(wrapped)
+      requires wrapped.consumed == [] && wrapped.produced == []
+      ensures Valid()
+    { 
+      this.filter := filter;
+      this.wrapped := wrapped;
+
+      consumed := [];
+      produced := [];
+      Repr := {this} + wrapped.Repr;
+      height := wrapped.height + 1;
+      wrappedCanProduce := wrapped.CanProduce;
+      new;
+      assert Enumerated(produced) == Seq.Filter(filter, Enumerated(wrapped.produced));
+    }
+
+    ghost predicate CanConsume(consumed: seq<()>, produced: seq<Option<T>>, next: ())
+      decreases height
+    {
+      true
+    }
+    ghost predicate CanProduce(consumed: seq<()>, produced: seq<Option<T>>)
+      decreases height
+    {
+      exists producedByWrapped: seq<Option<T>> ::
+        && wrappedCanProduce(Seq.Repeat((), |producedByWrapped|), producedByWrapped)
+        && Enumerated(produced) == Seq.Filter(filter, Enumerated(producedByWrapped))
+    }
+
+    method {:vcs_split_on_every_assert} Invoke(t: ()) returns (r: Option<T>) 
+      requires Valid()
+      requires CanConsume(consumed, produced, t)
+      modifies Repr
+      decreases height
+      ensures Valid()
+      ensures fresh(Repr - old(Repr))
+      ensures consumed == old(consumed) + [t]
+      ensures produced == old(produced) + [r]
+      ensures CanProduce(consumed, produced)
+    {
+      while true
+        invariant Valid()
+        invariant fresh(wrapped.Repr - old(wrapped.Repr))
+        invariant produced == old(produced)
+        invariant consumed == old(consumed)
+        invariant Enumerated(produced) == Seq.Filter(filter, Enumerated(wrapped.produced))
+        decreases EnumerationTerminationMetric(wrapped)
+      {
+        assert IsEnumerator(wrapped);
+        assert ConsumesAnything(wrapped);
+        assert wrapped.Valid();
+        assert wrapped.CanProduce(wrapped.consumed, wrapped.produced);
+        label before:
+        var r' := wrapped.Invoke(());
+
+        Repr := {this} + wrapped.Repr;
+        r := r';
+
+        if r.None? || filter(r.value) {
+          break;
+        }
+
+        var wrappedEnumeratedBefore := Enumerated(old@before(wrapped.produced));
+        assert wrapped.produced == old@before(wrapped.produced) + [r'];
+        assert Terminated(old@before(wrapped.produced), None, |old@before(wrapped.produced)|);
+        TerminatedDistributesOverConcat(old@before(wrapped.produced), [r], None, 1);
+        assert Enumerated(wrapped.produced) == wrappedEnumeratedBefore + [r.value];
+        LemmaFilterDistributesOverConcat(filter, wrappedEnumeratedBefore, [r.value]);
+        assert Enumerated(produced) == Seq.Filter(filter, Enumerated(wrapped.produced));
+
+        EnumerationTerminationMetricDecreased@before(wrapped, r);
+      }
+
+
+      Update(t, r);
+    }
+  }
+}
